\documentclass[a4paper,10pt]{article}
\usepackage[utf8x]{inputenc}

\usepackage{array}
\usepackage{graphicx}
\usepackage[sumlimits,intlimits,namelimits]{amsmath}
\usepackage{amssymb,amscd}

% \usepackage{courier}
\usepackage{amsmath}

\newcommand{\diff}[2]{\frac{\text{d} #1}{\text{d} #2}}



\begin{document}

\section{Aufgabe 5: Fehler bei Simpson}

\begin{align*}
E_n &= \frac{K_n}{(n+2)!} f^{n+2}(\xi) \\
K_n &= \int_a^b w_n(x) dx \\
w_n &= \prod_{i=0}^n (x-xi)
\end{align*}
mit $n = 2$ und $x_0 = a$, $x_1 = \frac{a+b}{2}, x_2 = b$
und der Transformation $t = \frac{x-a}{b-a}$ folgt
\begin{align*}
 x &= (b-a) t + a \\
 \Rightarrow \diff{x}{t} &= (b-a) \Rightarrow dx = dt (b - a) \\
\end{align*}
und
\begin{align*}
 x - a &= t(b - a)\\
 x - b &= t(b - a) + a - b = (t - 1)(b - a) \\
 x - \frac{a+b}{2} &= t(b - a) + a - \frac a 2 - \frac b 2 = t(b - a) + \frac a 2 - \frac b 2 = \left(t - \frac 1 2 \right)(b - a) \\
\end{align*}
Eingesetzt in $w_2$:
\begin{align*}
 w_2 = t\left(t - \frac 1 2\right) (t - 1) {(b - a)}^3
\end{align*}
Damit kann man das Integral $K_2$ auswerten:
\begin{align*}
 K_2(x) &= \int_a^b x t\left(t - \frac 1 2\right) (t - 1) {(b - a)}^3 dx
= \int_0^1 (t(b-a) + a) t\left(t - \frac 1 2\right) (t - 1) {(b - a)}^4 dt \\ 
&= {(b - a)}^4 \int_0^1 (t(b - a) + a)\left(t^2 - \frac 1 2 t\right)(t - 1) dt 
= {(b - a)}^4 \int_0^1 (t(b - a) + a) \left(t^3 - \frac 1 2 t - t^2 - \frac 1 2 t\right) dt \\
&= {(b - a)}^4 \int_0^1 \left(t^4 - \frac 1 2 t^3 - t^3 + \frac 1 2 t^2\right)(b - a) 
  + a t^3 - \frac 1 2 a t^2 - a t^2 + \frac 1 2 a t dt \\
&= {(b - a)}^4 \left[
  (b - a)\left(\frac 1 5 t^5 - \frac 1 4 t^4 - \frac 1 8 t^4 + \frac 1 6 t^3\right) + \frac 1 4 a t^4 - \frac 1 3 a t^3 - \frac 1 6 t^3 + \frac 1 4 a t^2
 \right]_0^1 \\\
&= {(b - a)}^4 \left[
  (b - a)\left(\frac 1 5 - \frac 1 4 - \frac 1 8 + \frac 1 6\right) + a \left(\frac 1 4 - \frac 1 3 - \frac 1 6 + \frac 1 4 \right)
\right] \\
&= {(b - a)}^4 \left[
(b - a) \left(\frac{8-5}{40} + \frac{4 - 6}{24} \right) + a \cdot 0
\right] \\
&= {(b - a)}^4 \left[
(b - a) \left(\frac{9}{120} - \frac{10}{120}\right)
\right] \\
&= - \frac{1}{120} {(b - a)}^5 \\
\end{align*}
Daraus folgt $E_2[f]$
\begin{align*}
 E_2[f] = - \frac{1}{120} {(b - a)}^5 \cdot \frac{1}{24} f^{n+2}(\xi) = - f^4{(\xi}) \frac{1}{90} \left(\frac{(b - a)}{2}\right)^5
\end{align*}






\end{document}
